partial proofs using discharge_simulationGeneral

prooftests/ExampleFromKamiTutorial_proofs.v
@@ -55,15 +55,170 @@ Proof.
   repeat split; auto; intros; unfold nthProp2; intros; try destruct (nth_error ls1 i) ; auto; repeat split; intros; try firstorder.
 Qed.
 
+Check flatten_inline_remove.
+
 Definition spec := (Foo'mod (mkProduceConsume (mkExtCall))).
-Definition impl := (flatten_inline_remove (HideMeth (Producer'mod (mkProducerConsumer (mkExtCall))) "send")).
+Definition impl := Base (flatten_inline_remove (HideMeth (Producer'mod (mkProducerConsumer (mkExtCall))) "send")).
 Hint Unfold spec : ModuleDefs.
 Hint Unfold impl : ModuleDefs.
+Check spec.
+Check impl.
 
-Theorem spec_impl_discharge_simulation (simRel: RegsT -> RegsT -> Prop):
-  TraceInclusion spec impl.
+Definition mySimRel (iregs sregs: RegsT) :=
+  (getKindAttr sregs = ("data", SyntaxKind (Bit 32)) :: nil)
+   /\ (getKindAttr iregs = ("data", SyntaxKind (Bit 32)) :: nil)
+   /\ Forall2 (fun (sreg ireg: RegT) => (fst sreg) = (fst ireg)) sregs iregs.
+
+Print makeBKModule.
+
+Definition flattened_spec := (BaseMod
+        (("data",
+         existT optConstFullT (SyntaxKind (Bit 32))
+           (Some (makeConst (ConstBit $0)))) :: nil)
+        (("produce",
+         fun ty : Kind -> Type =>
+         (Read ret : Bit 32 <- "data" ;
+          LETA _ : Void <-
+          LET v : Bit 32 <- Var ty (SyntaxKind (Bit 32)) ret ;
+          BKCall _ : Void <- "extCall"
+          (Var ty (SyntaxKind (Bit 32)) v : Bit 32) ;
+          Ret Const ty (ConstBit (wzero 0)) ;
+          Write "data" : Bit 32 <-
+          Var ty (SyntaxKind (Bit 32)) ret + Const ty (ConstBit $1) ;
+          Ret Const ty (ConstBit (wzero 0)))%kami_action) :: nil) nil).
+
+
+
+Definition flattened_impl :=
+(BaseMod
+        (("data",
+         existT optConstFullT (SyntaxKind (Bit 32))
+           (Some (makeConst (ConstBit $0)))) :: nil)
+        (("produce",
+         fun ty : Kind -> Type =>
+         (Read ret : Bit 32 <- "data" ;
+          LETA _ : Void <-
+          LET v : Bit 32 <- Var ty (SyntaxKind (Bit 32)) ret ;
+          BKCall _ : Void <- "extCall"
+          (Var ty (SyntaxKind (Bit 32)) v : Bit 32) ;
+          Ret Const ty (ConstBit (wzero 0)) ;
+          Write "data" : Bit 32 <-
+          Var ty (SyntaxKind (Bit 32)) ret + Const ty (ConstBit $1) ;
+          Ret Const ty (ConstBit (wzero 0)))%kami_action) :: nil) nil).
+
+Search (BaseModule -> BaseModuleWf).
+Definition flattened_spec_wf := {| baseModule := flattened_spec; wfBaseModule := ltac:(discharge_wf) |}.
+Definition flattened_impl_wf := {| baseModule := flattened_impl; wfBaseModule := ltac:(discharge_wf) |}.
+
+Theorem regs_ok:
+  forall x,
+  fst x = "data"
+  /\ projT1 (snd x) = SyntaxKind (Bit 32)
+  /\ exists rspec : list RegT,
+  Forall2
+    (fun (o' : RegT) (r : string * {x1 : FullKind & option (ConstFullT x1)}) =>
+     fst o' = fst r /\
+     (exists pf : projT1 (snd o') = projT1 (snd r),
+        match projT2 (snd r) with
+        | Some x1 =>
+            match pf in (_ = Y) return (fullType type Y) with
+            | eq_refl => projT2 (snd o')
+            end = evalConstFullT x1
+        | None => True
+        end)) rspec
+    (("data", existT optConstFullT (SyntaxKind (Bit 32)) (Some (makeConst (ConstBit $0))))
+     :: nil) /\ mySimRel (x :: nil) rspec.
+
 Proof.
-  do_inlining.
+Admitted.
 
+Theorem nodup_oimp:
+  forall oImp : RegsT, getKindAttr oImp = ("data", SyntaxKind (Bit 32)) :: nil -> NoDup (map fst oImp).
+Proof.
+Admitted.
+
+
+Theorem spec_spec_flattened_simulation:
+TraceInclusion
+  (Base
+     flattened_spec_wf)
+  (Base
+     flattened_spec_wf).
+Proof.
+  unfold flattened_impl_wf.
+  unfold flattened_impl.
+  unfold flattened_spec_wf.
+  unfold flattened_spec.
+  pose proof (wfBaseModule flattened_impl_wf) as wfImp.
+  discharge_simulationGeneral mySimRel (NoDup (map fst (getRegisters flattened_spec_wf))).
+  + discharge_NoSelfCall.
+  + unfold mySimRel in H. apply H.
+  + unfold mySimRel in H. apply H.
+  + intros. apply regs_ok.
+  + unfold mySimRel. econstructor.
+    unfold mySimRel in H1.
+    destruct H1. destruct H2. split.
+    * split.
+      ** apply H1.
+      ** split.
+         *** rewrite <- H2. rewrite <- getKindAttr_doUpdRegs. econstructor.
+          ++ apply nodup_oimp. apply H2.
+          ++ econstructor. eauto.
+             econstructor.
+          ++ intros. rewrite H2. econstructor. admit.
+         *** admit.
+    * admit. (* this one seems wrong *)
+Qed.
+
+Theorem spec_impl_flattened_simulation:
+TraceInclusion
+  (Base
+     flattened_impl_wf)
+  (Base
+     flattened_spec_wf).
+Proof.
+  unfold flattened_impl_wf.
+  unfold flattened_impl.
+  unfold flattened_spec_wf.
+  unfold flattened_spec.
+  pose proof (wfBaseModule flattened_impl_wf) as wfImp.
+  discharge_simulationGeneral mySimRel (NoDup (map fst (getRegisters flattened_impl_wf))).
+  + discharge_NoSelfCall.
+  + unfold mySimRel in H. apply H.
+  + unfold mySimRel in H. apply H.
+  + intros. apply regs_ok.
+  + unfold mySimRel. econstructor.
+    unfold mySimRel in H1.
+    destruct H1. destruct H2. split.
+    * split.
+      ** apply H1.
+      ** split.
+         *** rewrite <- H2. rewrite <- getKindAttr_doUpdRegs. econstructor.
+          ++ apply nodup_oimp. apply H2.
+          ++ econstructor. eauto.
+             econstructor.
+          ++ intros. rewrite H2. econstructor. admit.
+         *** admit.
+    * admit. (* this one seems wrong *)
+Qed.
+
+Theorem spec_impl_discharge_simulation:
+  TraceInclusion impl spec.
+Proof.
+  (* do_inlining. *)
+  unfold spec.
+  unfold mkProduceConsume.
+  unfold module'mkProduceConsume.mkProduceConsume.
+  unfold Foo'mod.
+  unfold module'mkProduceConsume.mkProduceConsumeModule.
+  unfold makeBKModule.
+  unfold makeBKModule'.
+  unfold concatModules.
+  repeat autounfold with ModuleDefs.
+
+  do_inlining.
+  pose proof (wfBaseModule imp) as wfImp.
+
+    apply simulationGeneral with (simRel := mySimRel). auto; simpl; intros.
   discharge_simulationGeneral simRel (NoDup (map fst (getRegisters impl))).
 Qed.
